https://oeis.org/A60724 Number of subgroups of the group C_n X C_n (where C_n is the cyclic group of order n).

https://oeis.org/A60724 : 1 5 6 15 8 30 10 37 23 40 14 90 16 50 48 83 20 115 22 120 60 70 26 222 45 80 76 150 32 240 34 177 84 100 80 345 40 110 96 296 44 300 46 210 184 130 50 498 75 225 120 240 56 380 112 370 132 160 62 720 64

size 194, time 5723922: loop2 ((loop (loop2 ((loop (loop2 (((loop2 ((if (((x * x) + x) mod y) <= 0 then (1 + y) else 1) + x) y (x - 1) 1 x) div x) * (if (y mod x) <= 0 then (1 + (y div x)) else 0)) 0 1 (1 - (loop (x - (if x <= 0 then 0 else y)) (1 + (2 + (2 + (x div (1 + (2 * (2 + 2))))))) (1 + x))) (loop (x - (if (y - x) <= 0 then y else 0)) (2 + (2 + (x div (1 + (2 * (2 + 2)))))) x)) 1 y) + x) (1 + y) x 0 (((x * x) - x) div 2)) 1 (loop (loop2 (if (y mod x) <= 0 then (1 + (y div x)) else 0) 0 1 (1 + (loop (x - (if (y - x) <= 0 then y else 0)) (2 + (2 + (x div (1 + (2 * (2 + 2)))))) x)) (1 - (loop (x - (if x <= 0 then 0 else y)) (1 + (2 + (2 + (x div (1 + (2 * (2 + 2))))))) (1 + x)))) 1 y)) + x) (1 + y) (x - (x div 2)) 1 (((x * x) - x) div 2)

K K F K D L H B L D B I K D L K B E B K N K G L K H B L K G D A I F A B B K K A L I E B C C K B C C C D F D G D D D B K D J E K L K E L A I E C C K B C C C D F D G D D K J N B L J K D B L D K A K K F K E C G N B L K H B L K G D A I A B B K L K E L A I E C C K B C C C D F D G D D K J D B K K A L I E B C C K B C C C D F D G D D D B K D J E N B L J J K D B L D K K C G E B K K F K E C G N

I think I can see a correspondence with one of the OEIS formulas. 
With mostly straightforward modifications (and one math problem :-) ), I can get it up to the attached code, 
and with a bit more insight I would agree it equals to Sum_{d|n} d\*tau((n/d)^2).

The analysis:

```
from itertools import islice

""" product of all the numbers of a given iterator
"""
def product(xs):
    res = 1
    for x in xs:
        res *= x
    return res

""" prime factorizartion
"""
def factorize(x):
    res = []
    p = 2
    while p*p <= x:        
        exp = 0
        while x % p == 0:
            x //= p
            exp += 1
        if exp: res.append((p,exp))
        p += 1
    if x != 1:
        res.append((x,1))
    return res

""" enumerates numbers as
    (0,0)
    (1,0), (1,1)
    (2,0), (2,1), (2,2)
    ...
"""
def triangle_index(x):
    y = 0
    while x > y:
        y += 1
        x -= y
    return y,x
def from_triangle_index(a,b):
    return b + a*(a+1)//2

for x in range(32):
    assert from_triangle_index(*triangle_index(x)) == x

""" number of solutions of x*(x+1) == 0 mod M
"""
def num_sol(M):
    return sum(
        1 for x in range(M)
        if x*(x+1) % M == 0
    )
# equality proof (link ANONYMIZED for IJCAI submission)
def num_sola(M):
    if M < 1: return 0
    return 2**(len(factorize(M)))

for x in range(1000):
    assert num_sol(x) == num_sola(x)

# matching with the original program

def f5(X):
    x,y = 1, X
    for z in range (1,(X - 1) + 1):
        x,y = (((1 + y) if (((x * x) + x) % y) <= 0 else 1) + x), y
    return x

def f5a(X):
    if X < 1: return 1
    return X*num_sola(X)

for x in range(1000):
    assert f5(x) == f5a(x)

def f6(X):
    x = 1 + X
    for y in range (1,(1 + (2 + (2 + (X // (1 + (2 * (2 + 2))))))) + 1):
        x = x - (0 if x <= 0 else y)
    return x
def f6a(X):
    a,b = triangle_index(X)
    return b-a

for x in range(1000):
    assert f6(x) == f6a(x)

def f7(X):
    x = X
    for y in range (1,(2 + (2 + (X // (1 + (2 * (2 + 2)))))) + 1):
        x = x - (y if (y - x) <= 0 else 0)
    return x
def f7a(X):
    a,b = triangle_index(X)
    return b

for x in range(1000):
    assert f7(x) == f7a(x)

def f4(X):
    x,y = 1 - f6(X), f7(X)
    for z in range (1,1 + 1):
        x,y = ((f5(x) // x) * ((1 + (y // x)) if (y % x) <= 0 else 0)), 0
    return x
def f4a(X):
    a,b = triangle_index(X)
    c = a-b+1
    if (b % c) == 0:
        return num_sola(c) * (1 + (b // c))
    else:
        return 0

for x in range(1000):
    assert f4(x) == f4a(x)
    
def f3(X,Y):
    x = Y
    for y in range (1,1 + 1):
        x = f4(x)
    return x
def f3a(X,Y):
    return f4(Y)

for x in range(32):
    for y in range(32):
        assert f3(x,y) == f3a(x,y)

def f2(X):
    x,y = 0, ((X * X) - X) // 2
    for z in range (1,X + 1):
        x,y = (f3(x,y) + x), (1 + y)
    return x
def f2a(X):
    return sum(
        num_sola(c) * (X // c)
        for c in range(1,X+1)
        if X % c == 0
    )

for x in range(32):
    assert f2(x) == f2a(x)    

def f10(X):
    x = X
    for y in range (1,(2 + (2 + (X // (1 + (2 * (2 + 2)))))) + 1):
        x = x - (y if (y - x) <= 0 else 0)
    return x
def f10a(X):
    a,b = triangle_index(X)
    return b

def f11(X):
    x = 1 + X
    for y in range (1,(1 + (2 + (2 + (X // (1 + (2 * (2 + 2))))))) + 1):
        x = x - (0 if x <= 0 else y)
    return x
def f11a(X):
    a,b = triangle_index(X)
    return b-a

for x in range(1000):
    assert f11(x) == f11a(x)

def f9(X):
    x,y = 1 + f10(X), 1 - f11(X)
    for z in range (1,1 + 1):
        x,y = ((1 + (y // x)) if (y % x) <= 0 else 0), 0
    return x
def f9a(X):
    a,b = triangle_index(X)
    if (a+2) % (b+1) == 0: return (a+2) // (b+1)
    else: return 0

for x in range(1000):
    assert f9(x) == f9a(x)

def f8(X,Y):
    x = Y
    for y in range (1,1 + 1):
        x = f9(x)
    return x
def f8a(X,Y):
    return f9a(Y)

for x in range(32):
    for y in range(32):
        assert f8(x,y) == f8a(x,y)

def f1(X,Y):
    x = f8(X,Y)
    for y in range (1,1 + 1):
        x = f2(x)
    return x
def f1a(X,Y):
    return f2a(f9a(Y))

for x in range(32):
    for y in range(32):
        assert f1(x,y) == f1a(x,y)

def f0(X):
    x,y = 1, ((X * X) - X) // 2
    for z in range (1,(X - (X // 2)) + 1):
        x,y = (f1(x,y) + x), (1 + y)
    return x
def f0a0(X):
    return 1 + sum(
        f2a( (X+1) // b)
        for b in range(1, (X+1) // 2 + 1)
        if (X+1) % b == 0
    )
def f0a1(X):
    return sum(
        sum(
            2**(len(factorize(c))) * (b // c)
            for c in range(1,b+1)
            if b % c == 0
        )
        for b in range(1, (X+2))
        if (X+1) % b == 0
    )
def f0a(X):
    return sum(
        sum(
            2**(len(factorize(c)))
            for c in range(1,b+1)
            if b % c == 0
        ) * ((X+1) // b)
        for b in range(1, (X+2))
        if (X+1) % b == 0
    )

for x in range(32):
    assert f0(x) == f0a0(x) # first version
    assert f0(x) == f0a1(x) # first version
    assert f0(x) == f0a(x)
    print (f0(x))

```



Original Python:

```
def f5(X):
    x,y = 1, X
    for z in range (1,(X - 1) + 1):
        x,y = (((1 + y) if (((x * x) + x) % y) <= 0 else 1) + x), y
    return x

def f6(X):
    x = 1 + X
    for y in range (1,(1 + (2 + (2 + (X // (1 + (2 * (2 + 2))))))) + 1):
        x = x - (0 if x <= 0 else y)
    return x

def f7(X):
    x = X
    for y in range (1,(2 + (2 + (X // (1 + (2 * (2 + 2)))))) + 1):
        x = x - (y if (y - x) <= 0 else 0)
    return x

def f4(X):
    x,y = 1 - f6(X), f7(X)
    for z in range (1,1 + 1):
        x,y = ((f5(x) // x) * ((1 + (y // x)) if (y % x) <= 0 else 0)), 0
    return x

def f3(X,Y):
    x = Y
    for y in range (1,1 + 1):
        x = f4(x)
    return x

def f2(X):
    x,y = 0, ((X * X) - X) // 2
    for z in range (1,X + 1):
        x,y = (f3(x,y) + x), (1 + y)
    return x

def f10(X):
    x = X
    for y in range (1,(2 + (2 + (X // (1 + (2 * (2 + 2)))))) + 1):
        x = x - (y if (y - x) <= 0 else 0)
    return x

def f11(X):
    x = 1 + X
    for y in range (1,(1 + (2 + (2 + (X // (1 + (2 * (2 + 2))))))) + 1):
        x = x - (0 if x <= 0 else y)
    return x

def f9(X):
    x,y = 1 + f10(X), 1 - f11(X)
    for z in range (1,1 + 1):
        x,y = ((1 + (y // x)) if (y % x) <= 0 else 0), 0
    return x

def f8(X,Y):
    x = Y
    for y in range (1,1 + 1):
        x = f9(x)
    return x

def f1(X,Y):
    x = f8(X,Y)
    for y in range (1,1 + 1):
        x = f2(x)
    return x

def f0(X):
    x,y = 1, ((X * X) - X) // 2
    for z in range (1,(X - (X // 2)) + 1):
        x,y = (f1(x,y) + x), (1 + y)
    return x

for x in range(32):
    print (f0(x))
```
